# Gegeben

$$
\begin{gather*}
	P_0 = (3, 2) \\
	P_1 = (0, ?) \\
	P_2 = (?, 0) \\
	m < 0
\end{gather*}
$$

# Geradengleichung

Die Gerade g sei definiert als $g(x) = mx + t$.

$$
\begin{alignat*}{2}
	&& y &= m \cdot x + t \\
	\iff&& 2 &= m \cdot 3 + t \\
	\iff&& t &= -3m + 2 \\
	\iff&& m &= \frac{2-t}{3} \\
\end{alignat*}
$$

# Dreiecksgleichung

$$
A = \frac{P_1^x \cdot P_2^y}{2}
$$

$$
\begin{align*}
	P_2^y &= g(0) = m \cdot 0 + t = t \\
	P_1^x &= -\frac{t}{m}
\end{align*}
$$

$$
\begin{align*}
	A &= -\frac{t \cdot \frac{t}{m}}{2} \\
	&= -\frac{t^2}{2m} \\
	&= -\frac{(-3m+2)^2}{2m} \\
	&= -\frac{4-12m+9m^2}{2m} \\
	&= -\frac{2}{m} - 6 + \frac{9}{2}m
\end{align*}
$$
