$$
(a - b)^2 = a^2 - 2ab + b^2
\tag{1}
$$

$$
\lim_{n \to \infty} \frac{a}{b} = \frac{\lim_{n \to \infty} a}{\lim_{n \to \infty} b}
\tag{2}
$$

$$
a_n \le b_n \le c_n \wedge \lim_{n \to \infty} a_n = \lim_{n \to \infty} c_n \implies \lim_{n \to \infty} b_n = \lim_{n \to \infty} a_n
\tag{3}
$$

$$
(a + b) \cdot (a - b) = a^2 - b^2
\tag{4}
$$

$$
(a + b)^n = \sum_{k=0}^{n} \binom{n}{k} a^{n-k} b^k
\tag{5}
$$

$$
\binom{n}{k} = \frac{n!}{k! \cdot (n-k)!}
\tag{6}
$$

$$
\sum_{k = k_0}^{n} f(k) = f(k_0) + \sum_{k = k_0 + 1}^{n} f(k)
\tag{7}
$$

$$
(1 - (1 - x)) = 1 - 1 + x = x
\tag{8}
$$

$$
\lim_{n \to \infty} a_n \pm b_n = a \pm b
\tag{9}
$$
